examples/wysteria/mill1.fst
@@ -17,10 +17,15 @@ let ab = union alice_s bob_s
 type pre  (m:mode)  = fun m0 -> b2t (m0 = m)
 type post (#a:Type) = fun (m:mode) (x:a) -> True
 
+val read_fn: unit -> Wys nat (fun m0 -> Mode.m m0 = Par /\
+                                        (exists p. Mode.ps m0 = singleton p))
+                             (fun m0 r -> True)
+let read_fn x = read #nat ()
+
 val mill1: unit -> Wys bool (pre (Mode Par ab)) post
 let mill1 _ =
- let x = as_par alice_s (read #nat) in
- let y = as_par bob_s (read #nat) in
+ let x = as_par alice_s read_fn in
+ let y = as_par bob_s read_fn in
 
  let g:unit -> Wys bool (pre (Mode Sec ab)) post =
    fun _ -> (unbox_s x) > (unbox_s y)
@@ -29,4 +34,5 @@ let mill1 _ =
  as_sec ab g
 ;;
 
-let _ = main ab mill1 in ()
+let x = main ab mill1 in
+wprint x
